viper-total-heaps/FoldStmtRelKF.thy
@@ -597,7 +597,7 @@ proof (rule stmt_rel_intro)
           apply (simp add: \<open>\<omega>1 = _\<close>)
          apply (simp add: \<open>\<omega>1 = _\<close>)
         apply (simp add: \<open>\<omega>1 = _\<close>)
-    using PredDecl WfCons \<open>Rep_preal (Abs_preal v_p) = p\<close> \<open>pbody' = pbody\<close> \<open>pdecl' = pdecl\<close> \<open>predicate_decl.body pdecl' = Some pbody'\<close> ctxt_pred_syn_wf_def prat_non_negative syntactic_mult_supported total_consistency_ctxt_wf(1)
+    using PredDecl WfCons CtxtPredWf \<open>Rep_preal (Abs_preal v_p) = p\<close> \<open>pbody' = pbody\<close> \<open>pdecl' = pdecl\<close> \<open>predicate_decl.body pdecl' = Some pbody'\<close> ctxt_pred_syn_wf_def prat_non_negative syntactic_mult_supported
        apply blast
     using BodyNoUnfolding
       apply auto[1]
@@ -936,7 +936,7 @@ next
              apply (rule \<open>\<omega>0 = _\<close>)+
            apply simp
           apply (rule v_args_eval)
-      using PredDecl WfCons \<open>Rep_preal (Abs_preal v_p) = p\<close> \<open>pbody' = pbody\<close> \<open>pdecl' = pdecl\<close> \<open>predicate_decl.body pdecl' = Some pbody'\<close> ctxt_pred_syn_wf_def prat_non_negative syntactic_mult_supported total_consistency_ctxt_wf(1)
+      using PredDecl WfCons CtxtPredWf \<open>Rep_preal (Abs_preal v_p) = p\<close> \<open>pbody' = pbody\<close> \<open>pdecl' = pdecl\<close> \<open>predicate_decl.body pdecl' = Some pbody'\<close> ctxt_pred_syn_wf_def prat_non_negative syntactic_mult_supported
          apply blast
       using BodyNoUnfolding
         apply auto[1]
